git/arthurpaulino/FunnyLang/lakefile.lean
@@ -1,6 +1,0 @@
-import Lake
-open Lake DSL
-
-package FunnyLang {
-  supportInterpreter := true
-}
