git/xubaiw/Unicode.lean/Unicode/Includes.lean
@@ -1,4 +1,3 @@
-import Lean
 import Mathlib.Util.IncludeStr
 import Std.Data.HashMap
 
@@ -15,20 +14,8 @@ namespace Unicode
 /-- Includes the ArabicShaping.txt string. -/
 def arabicShapingStr := include_str "../UCD/ArabicShaping.txt"
 
-/-- Includes the NamedSequences.txt string. -/
-def namedSequencesStr := include_str "../UCD/NamedSequences.txt"
-
 /-- Includes the BidiBrackets.txt string. -/
 def bidiBracketsStr := include_str "../UCD/BidiBrackets.txt"
-
-/-- Includes the NamedSequencesProv.txt string. -/
-def namedSequencesProvStr := include_str "../UCD/NamedSequencesProv.txt"
-
-/-- Includes the BidiCharacterTest.txt string. -/
-def bidiCharacterTestStr := include_str "../UCD/BidiCharacterTest.txt"
-
-/-- Includes the NamesList.txt string. -/
-def namesListStr := include_str "../UCD/NamesList.txt"
 
 /-- Includes the BidiMirroring.txt string. -/
 def bidiMirroringStr := include_str "../UCD/BidiMirroring.txt"
@@ -36,20 +23,11 @@ def bidiMirroringStr := include_str "../UCD/BidiMirroring.txt"
 /-- Includes the NormalizationCorrections.txt string. -/
 def normalizationCorrectionsStr := include_str "../UCD/NormalizationCorrections.txt"
 
-/-- Includes the BidiTest.txt string. -/
-def bidiTestStr := include_str "../UCD/BidiTest.txt"
-
-/-- Includes the NormalizationTest.txt string. -/
-def normalizationTestStr := include_str "../UCD/NormalizationTest.txt"
-
 /-- Includes the Blocks.txt string. -/
 def blocksStr := include_str "../UCD/Blocks.txt"
 
 /-- Includes the NushuSources.txt string. -/
 def nushuSourcesStr := include_str "../UCD/NushuSources.txt"
-
-/-- Includes the CJKRadicals.txt string. -/
-def cjkRadicalsStr := include_str "../UCD/CJKRadicals.txt"
 
 /-- Includes the PropList.txt string. -/
 def propListStr := include_str "../UCD/PropList.txt"
@@ -57,15 +35,9 @@ def propListStr := include_str "../UCD/PropList.txt"
 /-- Includes the CaseFolding.txt string. -/
 def caseFoldingStr := include_str "../UCD/CaseFolding.txt"
 
-/-- Includes the PropertyAliases.txt string. -/
-def propertyAliasesStr := include_str "../UCD/PropertyAliases.txt"
-
 /-- Includes the CompositionExclusions.txt string. -/
 def compositionExclusionsStr := include_str "../UCD/CompositionExclusions.txt"
   
-/-- Includes the PropertyValueAliases.txt string. -/
-def propertyValueAliasesStr := include_str "../UCD/PropertyValueAliases.txt"
-
 /-- Includes the DerivedAge.txt string. -/
 def derivedAgeStr := include_str "../UCD/DerivedAge.txt"
 
@@ -87,29 +59,14 @@ def specialCasingStr := include_str "../UCD/SpecialCasing.txt"
 /-- Includes the EastAsianWidth.txt string. -/
 def eastAsianWidthStr := include_str "../UCD/EastAsianWidth.txt"
 
-/-- Includes the StandardizedVariants.txt string. -/
-def standardizedVariantsStr := include_str "../UCD/StandardizedVariants.txt"
-
-/-- Includes the EmojiSources.txt string. -/
-def emojiSourcesStr := include_str "../UCD/EmojiSources.txt"
-
-/-- Includes the TangutSources.txt string. -/
-def tangutSourcesStr := include_str "../UCD/TangutSources.txt"
-
 /-- Includes the EquivalentUnifiedIdeograph.txt string. -/
 def equivalentUnifiedIdeographStr := include_str "../UCD/EquivalentUnifiedIdeograph.txt"
-
-/-- Includes the USourceData.txt string. -/
-def uSourceDataStr := include_str "../UCD/USourceData.txt"
 
 /-- Includes the HangulSyllableType.txt string. -/
 def hangulSyllableTypeStr := include_str "../UCD/HangulSyllableType.txt"
 
 /-- Includes the UnicodeData.txt string. See `unicodeDataMap`. -/
 def unicodeDataStr := include_str "../UCD/UnicodeData.txt"
-
-/-- Includes the Index.txt string. -/
-def indexStr := include_str "../UCD/Index.txt"
 
 /-- Includes the IndicPositionalCategory.txt string. -/
 def indicPositionalCategoryStr := include_str "../UCD/IndicPositionalCategory.txt"
@@ -136,23 +93,11 @@ def nameAliasesStr := include_str "../UCD/NameAliases.txt"
 /-- Includes the GraphemeBreakProperty.txt string. -/
 def graphemeBreakPropertyStr := include_str "../UCD/auxiliary/GraphemeBreakProperty.txt"
 
-/-- Includes the GraphemeBreakTest.txt string. -/
-def graphemeBreakTestStr := include_str "../UCD/auxiliary/GraphemeBreakTest.txt"
-
 /-- Includes the WordBreakProperty.txt string. -/
 def wordBreakPropertyStr := include_str "../UCD/auxiliary/WordBreakProperty.txt"
   
-/-- Includes the LineBreakTest.txt string. -/
-def lineBreakTestStr := include_str "../UCD/auxiliary/LineBreakTest.txt"
-
-/-- Includes the WordBreakTest.txt string. -/
-def wordBreakTestStr := include_str "../UCD/auxiliary/WordBreakTest.txt"
-
 /-- Includes the SentenceBreakProperty.txt string. -/
 def sentenceBreakPropertyStr := include_str "../UCD/auxiliary/SentenceBreakProperty.txt"
-
-/-- Includes the SentenceBreakTest.txt string. -/
-def sentenceBreakTestStr := include_str "../UCD/auxiliary/SentenceBreakTest.txt"
 
 /-!
   ### Emoji Subdirectory
@@ -161,75 +106,72 @@ def sentenceBreakTestStr := include_str "../UCD/auxiliary/SentenceBreakTest.txt"
 /-- Includes the emoji-data.txt string. -/
 def emojiDataStr := include_str "../UCD/emoji/emoji-data.txt"
 
-/-- Includes the emoji-variation-sequences.txt string. -/
-def emojiVariationSequencesStr := include_str "../UCD/emoji/emoji-variation-sequences.txt"
-
 /-!
   ### Extracted Subdirectory
 -/
 
-/-- Includes the SentenceBreakTest.txt string. -/
+/-- Includes the DerivedBidiClass.txt string. -/
 def derivedBidiClassStr := include_str "../UCD/extracted/DerivedBidiClass.txt"
 
-/-- Includes the SentenceBreakTest.txt string. -/
+/-- Includes the DerivedJoiningGroup.txt string. -/
 def derivedJoiningGroupStr := include_str "../UCD/extracted/DerivedJoiningGroup.txt"
 
-/-- Includes the SentenceBreakTest.txt string. -/
+/-- Includes the DerivedBinaryProperties.txt string. -/
 def derivedBinaryPropertiesStr := include_str "../UCD/extracted/DerivedBinaryProperties.txt"
 
-/-- Includes the SentenceBreakTest.txt string. -/
+/-- Includes the DerivedJoiningType.txt string. -/
 def derivedJoiningTypeStr := include_str "../UCD/extracted/DerivedJoiningType.txt"
 
-/-- Includes the SentenceBreakTest.txt string. -/
+/-- Includes the DerivedCombiningClass.txt string. -/
 def derivedCombiningClassStr := include_str "../UCD/extracted/DerivedCombiningClass.txt"
 
-/-- Includes the SentenceBreakTest.txt string. -/
+/-- Includes the DerivedLineBreak.txt string. -/
 def derivedLineBreakStr := include_str "../UCD/extracted/DerivedLineBreak.txt"
 
-/-- Includes the SentenceBreakTest.txt string. -/
+/-- Includes the DerivedDecompositionType.txt string. -/
 def derivedDecompositionTypeStr := include_str "../UCD/extracted/DerivedDecompositionType.txt"
 
-/-- Includes the SentenceBreakTest.txt string. -/
+/-- Includes the DerivedName.txt string. -/
 def derivedNameStr := include_str "../UCD/extracted/DerivedName.txt"
 
-/-- Includes the SentenceBreakTest.txt string. -/
+/-- Includes the DerivedEastAsianWidth.txt string. -/
 def derivedEastAsianWidthStr := include_str "../UCD/extracted/DerivedEastAsianWidth.txt"
 
-/-- Includes the SentenceBreakTest.txt string. -/
+/-- Includes the DerivedNumericType.txt string. -/
 def derivedNumericTypeStr := include_str "../UCD/extracted/DerivedNumericType.txt"
 
-/-- Includes the SentenceBreakTest.txt string. -/
+/-- Includes the DerivedGeneralCategory.txt string. -/
 def derivedGeneralCategoryStr := include_str "../UCD/extracted/DerivedGeneralCategory.txt"
 
-/-- Includes the SentenceBreakTest.txt string. -/
+/-- Includes the DerivedNumericValues.txt string. -/
 def derivedNumericValuesStr := include_str "../UCD/extracted/DerivedNumericValues.txt"
 
 /-!
   ### Unihan Subdirectory
 -/
 
-/-- Includes the SentenceBreakTest.txt string. -/
+/-- Includes the Unihan_DictionaryIndices.txt string. -/
 def unihanDictionaryIndicesStr := include_str "../UCD/Unihan/Unihan_DictionaryIndices.txt"
 
-/-- Includes the SentenceBreakTest.txt string. -/
+/-- Includes the Unihan_OtherMappings.txt string. -/
 def unihanOtherMappingsStr := include_str "../UCD/Unihan/Unihan_OtherMappings.txt"
 
-/-- Includes the SentenceBreakTest.txt string. -/
+/-- Includes the Unihan_DictionaryLikeData.txt string. -/
 def unihanDictionaryLikeDataStr := include_str "../UCD/Unihan/Unihan_DictionaryLikeData.txt"
 
-/-- Includes the SentenceBreakTest.txt string. -/
+/-- Includes the Unihan_RadicalStrokeCounts.txt string. -/
 def unihanRadicalStrokeCountsStr := include_str "../UCD/Unihan/Unihan_RadicalStrokeCounts.txt"
 
-/-- Includes the SentenceBreakTest.txt string. -/
+/-- Includes the Unihan_IRGSources.txt string. -/
 def unihanIRGSourcesStr := include_str "../UCD/Unihan/Unihan_IRGSources.txt"
 
-/-- Includes the SentenceBreakTest.txt string. -/
+/-- Includes the Unihan_Readings.txt string. -/
 def unihanReadingsStr := include_str "../UCD/Unihan/Unihan_Readings.txt"
 
-/-- Includes the SentenceBreakTest.txt string. -/
+/-- Includes the Unihan_NumericValues.txt string. -/
 def unihanNumericValuesStr := include_str "../UCD/Unihan/Unihan_NumericValues.txt"
 
-/-- Includes the SentenceBreakTest.txt string. -/
+/-- Includes the Unihan_Variants.txt string. -/
 def unihanVariantsStr := include_str "../UCD/Unihan/Unihan_Variants.txt"
 
 /-!
@@ -246,22 +188,224 @@ private def decodeHex! (s : String) : Nat :=
     | '5' => 5 | '6' => 6 | '7' => 7 | '8' => 8 | '9' => 9
     | 'a' => 10 | 'b' => 11 | 'c' => 12 | 'd' => 13 | 'e' => 14 | 'f' => 15
     | 'A' => 10 | 'B' => 11 | 'C' => 12 | 'D' => 13 | 'E' => 14 | 'F' => 15
-    | _ => panic! "Invalid hex digit"
+    | c => panic! s!"Invalid hex digit {c}"
     foldlHexDigits acc d := 16 * acc + d
 
 /-- Make `Char` `Hashable` as key of `HashMap`. -/
-instance : Hashable Char := ⟨ λ c => String.hash $ Char.toString c ⟩ 
-
+instance : Hashable Char := ⟨ λ c => String.hash $ toString c ⟩ 
 /-- Parse data file `String` into `HashMap`, the unit in parameter is left for `Thunk`. -/
-def parseStrToMapFn (s : String) (unit : Unit) : HashMap Char (List String) := Id.run do
-  let mut map := HashMap.empty
-  for line in unicodeDataStr.splitOn "\n" |>.filter (· ≠ "") do
-    let splits := line.splitOn ";" |>.map String.trim
-    let char := Char.ofNat $ decodeHex! $ splits.get! 0
-    map := map.insert char (splits.tail!)
-  return map
+def parseStrToMapFn (s : String) (unit : Unit) : HashMap Char (List String)  := Id.run do
+  let mut rangeStarts := HashMap.empty
+  let mut result := .empty
+  for line in s.splitOn "\n" |>.filterMap lineCleanup do
+    let splits := line.splitOn ";" |>.map (·.splitOn "\t") |>.join |>.map String.trim
+    let first := splits.head! |>.replace "U+" ""
+    -- range
+    if first.contains '.' then
+      let splits := first.splitOn ".."
+      let start := decodeHex! splits.head!
+      let stop := decodeHex! splits.getLast!
+      for val in [start:(stop+1)] do
+        result := result.insert (.ofNat val) (splits.tail!)
+    -- mutiple
+    else if first.contains ' ' then
+      let splits := first.splitOn " "
+      for val in splits do
+        result := result.insert (.ofNat $ decodeHex! val) (splits.tail!)
+    else
+      if let some second := splits.get? 1 then
+        -- backward range start
+        if second.endsWith ", First>" then
+          let name := second |>.replace ", First>" "" |>.replace "<" ""
+          rangeStarts := rangeStarts.insert name (decodeHex! first)
+        -- backward range end
+        else if second.endsWith ", Last>" then
+          let name := second |>.replace ", Last>" "" |>.replace "<" ""
+          let start := rangeStarts.find! name
+          let stop := decodeHex! first
+          let newTail := name::splits.tail!.tail!
+          for val in [start:(stop+1)] do
+            result := result.insert (.ofNat val) newTail
+        -- single
+        else
+          result := result.insert (.ofNat $ decodeHex! first) (splits.tail!)
+      -- single
+      else
+        result := result.insert (.ofNat $ decodeHex! first) (splits.tail!)
+  return result
+where
+  /-- Remove comments and empty lines. -/
+  lineCleanup (line : String) : Option String :=
+    line.splitOn "#"
+    |>.head?
+    |>.filter (·.trim ≠ "")
 
-/-- Includes the UnicodeData.txt data. -/
-def unicodeDataMap : Thunk (HashMap Char (List String)) := ⟨ parseStrToMapFn unicodeDataStr ⟩ 
+/-!
+  ### UCD Main Directory
+-/
+
+/-- Includes the ArabicShaping.txt data. -/
+def arabicShapingMap := Thunk.mk $ parseStrToMapFn arabicShapingStr
+
+/-- Includes the BidiBrackets.txt data. -/
+def bidiBracketsMap := Thunk.mk $ parseStrToMapFn bidiBracketsStr
+
+/-- Includes the BidiMirroring.txt data. -/
+def bidiMirroringMap := Thunk.mk $ parseStrToMapFn bidiMirroringStr
+
+/-- Includes the NormalizationCorrections.txt data. -/
+def normalizationCorrectionsMap := Thunk.mk $ parseStrToMapFn normalizationCorrectionsStr
+
+/-- Includes the Blocks.txt data. -/
+def blocksMap := Thunk.mk $ parseStrToMapFn blocksStr
+
+/-- Includes the NushuSources.txt data. -/
+def nushuSourcesMap := Thunk.mk $ parseStrToMapFn nushuSourcesStr
+
+/-- Includes the PropList.txt data. -/
+def propListMap := Thunk.mk $ parseStrToMapFn propListStr
+
+/-- Includes the CaseFolding.txt data. -/
+def caseFoldingMap := Thunk.mk $ parseStrToMapFn caseFoldingStr
+
+/-- Includes the CompositionExclusions.txt data. -/
+def compositionExclusionsMap := Thunk.mk $ parseStrToMapFn compositionExclusionsStr
+  
+/-- Includes the DerivedAge.txt data. -/
+def derivedAgeMap := Thunk.mk $ parseStrToMapFn derivedAgeStr
+
+/-- Includes the ScriptExtensions.txt data. -/
+def scriptExtensionsMap := Thunk.mk $ parseStrToMapFn scriptExtensionsStr
+
+/-- Includes the DerivedCoreProperties.txt data. -/
+def derivedCorePropertiesMap := Thunk.mk $ parseStrToMapFn derivedCorePropertiesStr
+
+/-- Includes the Scripts.txt data. -/
+def scriptsMap := Thunk.mk $ parseStrToMapFn scriptsStr
+
+/-- Includes the DerivedNormalizationProps.txt data. -/
+def derivedNormalizationPropsMap := Thunk.mk $ parseStrToMapFn derivedNormalizationPropsStr
+
+/-- Includes the SpecialCasing.txt data. -/
+def specialCasingMap := Thunk.mk $ parseStrToMapFn specialCasingStr
+
+/-- Includes the EastAsianWidth.txt data. -/
+def eastAsianWidthMap := Thunk.mk $ parseStrToMapFn eastAsianWidthStr
+
+/-- Includes the EquivalentUnifiedIdeograph.txt data. -/
+def equivalentUnifiedIdeographMap := Thunk.mk $ parseStrToMapFn equivalentUnifiedIdeographStr
+
+/-- Includes the HangulSyllableType.txt data. -/
+def hangulSyllableTypeMap := Thunk.mk $ parseStrToMapFn hangulSyllableTypeStr
+
+/-- Includes the UnicodeData.txt data. See `unicodeDataMap`. -/
+def unicodeDataMap := Thunk.mk $ parseStrToMapFn unicodeDataStr
+
+/-- Includes the IndicPositionalCategory.txt data. -/
+def indicPositionalCategoryMap := Thunk.mk $ parseStrToMapFn indicPositionalCategoryStr
+
+/-- Includes the VerticalOrientation.txt data. -/
+def verticalOrientationMap := Thunk.mk $ parseStrToMapFn verticalOrientationStr
+
+/-- Includes the IndicSyllabicCategory.txt data. -/
+def indicSyllabicCategoryMap := Thunk.mk $ parseStrToMapFn indicSyllabicCategoryStr
+
+/-- Includes the Jamo.txt data. -/
+def jamoMap := Thunk.mk $ parseStrToMapFn jamoStr
+
+/-- Includes the LineBreak.txt data. -/
+def lineBreakMap := Thunk.mk $ parseStrToMapFn lineBreakStr
+
+/-- Includes the NameAliases.txt data. -/
+def nameAliasesMap := Thunk.mk $ parseStrToMapFn nameAliasesStr
+
+/-!
+  ### Auxiliary Subdirectory
+-/
+
+/-- Includes the GraphemeBreakProperty.txt data. -/
+def graphemeBreakPropertyMap := Thunk.mk $ parseStrToMapFn graphemeBreakPropertyStr
+
+/-- Includes the WordBreakProperty.txt data. -/
+def wordBreakPropertyMap := Thunk.mk $ parseStrToMapFn wordBreakPropertyStr
+  
+/-- Includes the SentenceBreakProperty.txt data. -/
+def sentenceBreakPropertyMap := Thunk.mk $ parseStrToMapFn sentenceBreakPropertyStr
+
+/-!
+  ### Emoji Subdirectory
+-/
+
+/-- Includes the emoji-data.txt data. -/
+def emojiDataMap := Thunk.mk $ parseStrToMapFn emojiDataStr
+
+/-!
+  ### Extracted Subdirectory
+-/
+
+/-- Includes the DerivedBidiClass.txt string. -/
+def derivedBidiClassMap := Thunk.mk $ parseStrToMapFn derivedBidiClassStr
+
+/-- Includes the DerivedJoiningGroup.txt string. -/
+def derivedJoiningGroupMap := Thunk.mk $ parseStrToMapFn derivedJoiningGroupStr
+
+/-- Includes the DerivedBinaryProperties.txt string. -/
+def derivedBinaryPropertiesMap := Thunk.mk $ parseStrToMapFn derivedBinaryPropertiesStr
+
+/-- Includes the DerivedJoiningType.txt string. -/
+def derivedJoiningTypeMap := Thunk.mk $ parseStrToMapFn derivedJoiningTypeStr
+
+/-- Includes the DerivedCombiningClass.txt string. -/
+def derivedCombiningClassMap := Thunk.mk $ parseStrToMapFn derivedCombiningClassStr
+
+/-- Includes the DerivedLineBreak.txt string. -/
+def derivedLineBreakMap := Thunk.mk $ parseStrToMapFn derivedLineBreakStr
+
+/-- Includes the DerivedDecompositionType.txt string. -/
+def derivedDecompositionTypeMap := Thunk.mk $ parseStrToMapFn derivedDecompositionTypeStr
+
+/-- Includes the DerivedName.txt string. -/
+def derivedNameMap := Thunk.mk $ parseStrToMapFn derivedNameStr
+
+/-- Includes the DerivedEastAsianWidth.txt string. -/
+def derivedEastAsianWidthMap := Thunk.mk $ parseStrToMapFn derivedEastAsianWidthStr
+
+/-- Includes the DerivedNumericType.txt string. -/
+def derivedNumericTypeMap := Thunk.mk $ parseStrToMapFn derivedNumericTypeStr
+
+/-- Includes the DerivedGeneralCategory.txt string. -/
+def derivedGeneralCategoryMap := Thunk.mk $ parseStrToMapFn derivedGeneralCategoryStr
+
+/-- Includes the DerivedNumericValues.txt string. -/
+def derivedNumericValuesMap := Thunk.mk $ parseStrToMapFn derivedNumericValuesStr
+
+/-!
+  ### Unihan Subdirectory
+-/
+
+/-- Includes the Unihan_DictionaryIndices.txt string. -/
+def unihanDictionaryIndicesMap := Thunk.mk $ parseStrToMapFn unihanDictionaryIndicesStr
+
+/-- Includes the Unihan_OtherMappings.txt string. -/
+def unihanOtherMappingsMap := Thunk.mk $ parseStrToMapFn unihanOtherMappingsStr
+
+/-- Includes the Unihan_DictionaryLikeData.txt string. -/
+def unihanDictionaryLikeDataMap := Thunk.mk $ parseStrToMapFn unihanDictionaryLikeDataStr
+
+/-- Includes the Unihan_RadicalStrokeCounts.txt string. -/
+def unihanRadicalStrokeCountsMap := Thunk.mk $ parseStrToMapFn unihanRadicalStrokeCountsStr
+
+/-- Includes the Unihan_IRGSources.txt string. -/
+def unihanIRGSourcesMap := Thunk.mk $ parseStrToMapFn unihanIRGSourcesStr
+
+/-- Includes the Unihan_Readings.txt string. -/
+def unihanReadingsMap := Thunk.mk $ parseStrToMapFn unihanReadingsStr
+
+/-- Includes the Unihan_NumericValues.txt string. -/
+def unihanNumericValuesMap := Thunk.mk $ parseStrToMapFn unihanNumericValuesStr
+
+/-- Includes the Unihan_Variants.txt string. -/
+def unihanVariantsMap := Thunk.mk $ parseStrToMapFn unihanVariantsStr
 
 end Unicode
+
